wip! revision

Lp2lc/Active/Dot/Def.lean
@@ -7,11 +7,11 @@ namespace Lp2lc.Active.Dot
 
 /-
 here is the self-contained syntax for the latest DOT (System D-Diamond with
-object/record, with real forAll).
+object/record, with real ∀).
 
 It is:
 
-- Not System F! (or its extension, lack of explicit polyFn, polyArrow, fake forAll)
+- Not System F! (or its extension, lack of explicit polyFn, polyArrow, fake ∀)
 - Not WadlerFest 2016 version! (lack of union type)
 -/
 
@@ -49,28 +49,31 @@ def ByteCode := String
 
 abbrev Label := String
 
-abbrev LookupFn (V : Type) := Label → Option V
-
 section
 
-variable (V : Type)
+variable {Key : Type} {V : Type}
 
-namespace LookupFn
+abbrev Lookup := Key → Option V
 
-def empty : LookupFn V := fun _ => none
+namespace Lookup
 
-def set (σ : LookupFn V) (x : Label) (v : V) : LookupFn V :=
+def empty : Lookup (Key := Key) (V := V) := fun _ => none
+
+def set [DecidableEq Key] (σ : Lookup (Key := Key) (V := V)) (x : Key) (v : V) :
+    Lookup (Key := Key) (V := V) :=
   fun y => if y = x then some v else σ y
 
-@[simp] theorem set_same (σ : LookupFn V) (x : Label) (v : V) :
-  LookupFn.set (V := V) σ x v x = some v := by
-  simp [LookupFn.set]
+@[simp] theorem set_same [DecidableEq Key] (σ : Lookup (Key := Key) (V := V)) (x : Key)
+    (v : V) :
+  set σ x v x = some v := by
+  simp [set]
 
-@[simp] theorem set_other (σ : LookupFn V) (x y : Label) (v : V) (h : y ≠ x) :
-  LookupFn.set (V := V) σ x v y = σ y := by
-  simp [LookupFn.set, h]
+@[simp] theorem set_other [DecidableEq Key] (σ : Lookup (Key := Key) (V := V)) (x y : Key)
+    (v : V) (h : y ≠ x) :
+  set σ x v y = σ y := by
+  simp [set, h]
 
-end LookupFn
+end Lookup
 
 structure ObjectBody (V : Type) where
   underlying : Label → Option V
@@ -83,20 +86,20 @@ variable (I: Type)[DecidableEq I] -- index
 
 mutual
 
-inductive Entry: Type where -- member of an object
+inductive Entry: Type where -- member of an object/record
 | type (tLabel: Label) (ty: Typ) : Entry -- `{type Label = Ty}`
 | term (label: Label) (tm: Trm) : Entry -- `{term label = Tm}`
 
 inductive Typ : Type where
 -- | later (raw: Typ) : Typ -- don't know how to use it in iris yet.
 | primitive : Typ -- `AnyVal`, won't differentiate Int/Float/Byte.
+| depFn (tIn : Typ) (tOut: Typ) : Typ -- function `In => Out` or dependent function (if `tOut` is a "depSelectTyp")
 | subtypeEv (tUnder: Typ) (tOver: Typ) : Typ -- subtype evidence, AKA coercion, `Under <:< Over`
-| depFn (tIn : Typ) (tOut: Typ) : Typ -- function (`In => Out`) or dependent function (if `tOut` is a "depSelectTyp")
-| object1 (entry : Entry) : Typ -- AKA record1, only has 1 member
--- TODO: this hasn't been defined in PHOAS before, need to double check.
--- Kind of hairy, how could object I be available when the object body is half-defined?
-| depSelectTyp (object: I) (tK: Label) : Typ -- `object.Label` -- (object: I) used to be a de Bruijn serial which is 0 for `this.K`, in PHOAS we have to use Trm.self
-| self (self: Typ) : Typ -- AKA type binding, Mu-type, `this`
+| entry (single : Entry) : Typ -- AKA object1, record1, 1 member only
+-- TODO: this hasn't been defined in PHOAS before, need more sanity check.
+| depSelectTyp (object: I) (tK: Label) : Typ -- `object.Label`
+| selfBinder (self: Typ) : Typ -- AKA Mu-type, the delimiter/wrapper in an AST of which "Trm.self" refers to
+| singleton (v: Trm) : Typ -- path singleton type that can only bind `v`, `v.type`
 | and (tX: Typ) (tY: Typ) : Typ -- AKA intersection, `X & Y`
 | or (tX: Typ) (tY: Typ) : Typ -- AKA union, `X | Y`
 | top  : Typ -- `Any`
@@ -104,32 +107,56 @@ inductive Typ : Type where
 
 inductive Val : Type where -- evaluation results and args of Atomic Normal Form (ANF), `Typ` CANNOT be carried! they are erased at runtime!
 | primitive : Val -- `3`, `3.2`, `true` etc.
-| object (lookup : ObjectBody Entry) : Val -- carrying a member lookup, in DOT objects are only identified only by structure, Trait has to carry a hidden type member
-| depFn (body : (arg: I) -> Trm) : Val -- same as Typ
--- TODO: do we need typing evidence?
--- TODO: for operational semantics, Val should be indistinguisable from denotation, in the next version they should be unified (if positivity doesn't block it)
+| object (lookup : ObjectBody Entry) : Val -- carrying a member lookup, DOT only uses structural typing so Trait has to carry an extra hidden type member
+| depFn (body : (arg: I) -> Trm) : Val -- see "Typ.depFn"
+| subtypeEv : Val -- see "Typ.subtypeEv", has no body, erased at runtime
 
 inductive Trm : Type where -- AKA expression, unlike Val, it is indexed by type
-| var (symbol: I) : Trm -- `x`
-| val (v : Val) : Trm -- AKA literal, Values are terms
-| self : Trm -- AKA self-binder, `this`
+| var (symbol: I) : Trm -- variable, `x`, always bounded, almost always locally closed (In PHOAS it is imposible to construct wildcard "(symbol: I)")
+| val (v : Val) : Trm -- value, AKA literal
+| self : Trm -- self-var, `this`, must be inside a "Typ.selfBinder". If de Bruijn serial is used for bounded var then this is the "0".
 | depSelectTrm (object: I) (label: Label) : Trm  -- `object.label`
 | depApply (fn: Trm) (arg: Trm) : Trm -- application of (dependent?) function
-| subtypeEv : Trm -- same as Typ, has no coercion body, erased at runtime
+
+-- TODO: some of these can be merged actually, e.g. subtypeEv and depFn
 
 end
+
+namespace postpone -- DOT with type constructors/generics with type bound & variance, fully defined Scala.
+-- TODO: eventually this part has to be added with examples, including
+-- elaborator rules
+
+inductive TypCtor : Type where -- type constructor! not type! not in core DOT!
+| ctor: (arg : I -> Typ I) -> TypCtor
+
+end postpone
+
+/-
+Semantics
+TODO: each constraint has 2 semantic representation:
+
+- embedded/definitional: type bindings are predicates for terms (Trm -> Prop), subtype
+  evidences are higher-order predicates:
+  ∀ {T1 T2 : Trm -> Prop} {v : Trm} (ev: T1 <:< T2) (T1 v) -> (T2 v)
+- explicit/operational: type bindings are lookup, subtype evidences are lattice, both forms
+  the Env/Context
+
+they don't have to match, but which one would you choose?
+-/
+
+/-
+if choosing embedded/definitional:
+
+Some Val should be indistinguisable from denotation, (all of them if positivity
+doesn't block it), can we avoid repetitive definitions?
+-/
 
 -- inductive Data: Type where -- AKA Denotation
 -- | primitive : Data -- `3`, `3.2`, `true` etc.
 -- | object : (Lookup Data or (Data -> Data) ) → Data -- carrying a member lookup, in DOT objects are only identified only by structure, Trait has to carry a hidden type member
 
 
-namespace postpone
 
-inductive TypCtor : Type where -- type constructor! not type! not in core DOT!
-| ctor: (arg : I -> Typ I) -> TypCtor
-
-end postpone
 
 end Syntax
 
